Modules/TypeSystem/TypesAreOmegaGroupoids/InhabitRelation.v
@@ -1,0 +1,452 @@
+
+(* -*- coq-prog-name: "coqtop"; -*- *)
+Require Import ssreflect ssrfun ssrbool .
+
+Require Import Coq.Logic.JMeq.
+From Modules Require Import PreSyntaxOnlyContr libhomot lib WfSyntaxBrunerieOnlyContr FunctionalRelation.
+Set Bullet Behavior "Strict Subproofs".
+
+Set Implicit Arguments.
+Unset Strict Implicit.
+Unset Printing Implicit Defensive.
+
+Section TypeRl.
+  Variable (T: Type).
+  Variable (fibT: Fib T).
+
+Record rfC (Γ : Con) (wΓ : WC Γ) :=
+  { fC_C : rC T ;
+    fC_r : rl_C fibT wΓ fC_C
+  }.
+
+Record rfT (Γ : Con) (A : Ty) (wΓ : WC Γ) (wA : (Γ ⊢ A)) :=
+  { fT_C : rC T;
+    fT_T : rT fT_C;
+    fT_r : rl_T fibT wΓ wA (mkpT fT_T)
+  }.
+
+Record rft (Γ : Con) (A : Ty) (t : Tm) (wΓ : WC Γ) (wA : (Γ ⊢ A)) (wt : Γ ⊢ t : A) :=
+  { ft_C : rC T;
+    ft_T : rT ft_C;
+    ft_t : rtm ft_T;
+    ft_r :  rl_t fibT wΓ wA wt (mkpt ft_t );
+    (* ft_rT :  rl_T fibT wΓ wA (mkpT ft_T)  *)
+  }.
+Definition ft_rT (Γ : Con) (A : Ty) (t : Tm) (wΓ : WC Γ) (wA : (Γ ⊢ A)) (wt : Γ ⊢ t : A)
+      (ft : rft wΓ wA wt) : rl_T fibT wΓ wA (mkpT (ft_T ft)) := rl_t_Tη (ft_r ft).
+
+Record rfV (Γ : Con) (A : Ty) (x : Var) (wΓ : WC Γ) (wA : (Γ ⊢ A)) (wx : WVar Γ A x) :=
+  { fV_C : rC T;
+    fV_T : rT fV_C;
+    fV_t : rtm fV_T;
+    fV_r :  rl_V fibT wΓ wA wx (mkpt fV_t );
+    (* fV_rT :  rl_T fibT wΓ wA (mkpT fV_T) ; *)
+    (* fV_rC T :  rl_C fibT wΓ fV_C  *)
+  }.
+Definition fV_rT (Γ : Con) (A : Ty) (x:Var) (wΓ : WC Γ) (wA : (Γ ⊢ A)) ( wx : WVar Γ A x)
+      (fx : rfV wΓ wA wx) : rl_T fibT wΓ wA (mkpT (fV_T fx)) := rl_V_Tη (fV_r fx).
+Definition fV_rC  (Γ : Con) (A : Ty) (x:Var) (wΓ : WC Γ) (wA : (Γ ⊢ A)) ( wx : WVar Γ A x)
+      (fx : rfV wΓ wA wx) : rl_C fibT wΓ  ((fV_C fx)) := rl_V_Cη (fV_r fx).
+
+Record rfS (Γ Δ : Con) (σ : sub) (wΓ : WC Γ) (wΔ : WC Δ) (wσ : Γ ⊢ σ ⇒ Δ) :=
+  { fS_Γ : rC T;
+    fS_Δ : rC T;
+    fS_S : rS fS_Γ fS_Δ;
+    fS_r : rl_S fibT wΓ wΔ wσ (mkpS fS_S)}.
+
+
+  Lemma eqf_CC_TC (Γ : Con) (A : Ty) (wΓ : WC Γ) (wA : Γ ⊢ A)
+        (fΓ : rfC wΓ) (fA : rfT wΓ wA) : fC_C fΓ = fT_C fA.
+  Proof.
+    apply:rl_hpC.
+    + apply:fC_r.
+    + apply:rl_T_Cη.
+      apply:fT_r.
+  Qed.
+  Lemma eqf_tC_TC (Γ : Con) (A : Ty) t (wΓ : WC Γ) (wA : Γ ⊢ A) (wt : Γ ⊢ t : A)
+         (fA : rfT wΓ wA)(ft : rft wΓ wA wt) : ft_C ft = fT_C fA .
+  Proof.
+    apply:rl_hpC.
+    + apply:rl_t_Cη. 
+      apply:ft_r.
+    + apply:rl_T_Cη.
+      apply:fT_r.
+  Qed.
+  
+  Lemma eqf_tC_tC (Γ : Con) (A : Ty) t u (wΓ : WC Γ) (wA : Γ ⊢ A) (wt : Γ ⊢ t : A)
+        (wu : Γ ⊢ u : A)
+         (ft : rft wΓ wA wt)(fu : rft wΓ wA wu) : ft_C ft = ft_C fu .
+  Proof.
+    apply:rl_hpC.
+    + apply:(rl_t_Cη).
+      apply:ft_r.
+    + apply:(rl_t_Cη).
+      apply:ft_r.
+  Qed.
+  Lemma eqf_tT_tT (Γ : Con) (A : Ty) t u (wΓ : WC Γ) (wA : Γ ⊢ A) (wt : Γ ⊢ t : A)
+        (wu : Γ ⊢ u : A)
+         (ft : rft wΓ wA wt)(fu : rft wΓ wA wu) : ft_T ft ≅ ft_T fu .
+  Proof.
+    apply:π_eq_pTη'.
+    apply:rl_hpT.
+    + apply:ft_rT.
+    + apply:ft_rT.
+  Qed.
+  Lemma eqf_tT_TT (Γ : Con) (A : Ty) t (wΓ : WC Γ) (wA : Γ ⊢ A) (wt : Γ ⊢ t : A)
+         (fA : rfT wΓ wA)(ft : rft wΓ wA wt) : ft_T ft ≅ fT_T fA .
+  Proof.
+    apply:π_eq_pTη'.
+    apply:rl_hpT.
+    + apply:ft_rT.
+    + apply:fT_r.
+  Qed.
+  Lemma eqf_SC1_CC (Γ : Con)  (wΓ : WC Γ) 
+        (Δ : Con) (wΔ : WC Δ) (σ : sub) (wσ : Γ ⊢ σ ⇒ Δ)
+        (fΓ : rfC wΓ)(fσ : rfS wΓ wΔ wσ) :
+    fS_Γ fσ = fC_C fΓ.
+  Proof.
+    apply:rl_hpC.
+    + apply:(rl_S_C1 (pσ := mkpS (fS_S fσ))).
+      apply:fS_r.
+    + apply:fC_r.
+  Qed.
+  Lemma eqf_SC2_CC (Γ : Con)  (wΓ : WC Γ) 
+        (Δ : Con) (wΔ : WC Δ) (σ : sub) (wσ : Γ ⊢ σ ⇒ Δ)
+        (fΔ : rfC wΔ)(fσ : rfS wΓ wΔ wσ) :
+    fS_Δ fσ = fC_C fΔ.
+  Proof.
+    apply:rl_hpC.
+    + apply:(rl_S_C2 (pσ := mkpS (fS_S fσ))).
+      apply:fS_r.
+    + apply:fC_r.
+  Qed.
+
+Fixpoint semC (Γ : Con) (wΓ : WC Γ) {struct wΓ} : rfC wΓ
+with semT (Γ : Con) (A : Ty) (wΓ : WC Γ) (wA : Γ ⊢ A) : rfT wΓ wA
+with semt  (Γ : Con)  (A : _) (t : Tm)
+             (wΓ : WC Γ)(wA : Γ ⊢ A) (wt : Γ ⊢ t : A) : rft wΓ wA wt
+with semV  (Γ : Con)  (A : _) (x : Var)
+           (wΓ : WC Γ)
+           (wA : Γ ⊢ A)
+           (wx : WVar Γ A x) : rfV wΓ wA wx
+with semS (Γ Δ : Con)  (σ : sub)
+            (wΓ : WC Γ)(wΔ : WC Δ) (wσ : Γ ⊢ σ ⇒ Δ) : rfS wΓ wΔ wσ .
+- destruct wΓ.
+  + unshelve econstructor.
+    * apply :r_rl_astar => //.
+    * constructor.
+  + specialize (semt _ _ _ wΓ w w0).
+    unshelve econstructor.
+    * apply:r_rl_ext.
+      apply:(ft_t semt).
+    * constructor => //.
+      -- apply:(rl_t_C (ft_r semt)).
+      -- apply:ft_rT.
+      -- apply:ft_r.
+- destruct wA.
+  + specialize (semC _ w).
+    unshelve econstructor.
+    * exact (fC_C semC).
+    * apply:r_rl_star=> //.
+    * abstract (clear_hprop; by move/rl_star:(fC_r semC)).
+  + specialize (semT _ _ wΓ wA).
+    have st := (semt _ _ _ wΓ wA w).
+    have su := (semt _ _ _ wΓ wA w0).
+    unshelve econstructor.
+    * apply:ft_C.
+      exact:st.
+    * apply:r_rl_ar.
+      -- apply:ft_t.
+      -- move: (ft_t su).
+         apply:transport2.
+         ** apply:eqf_tC_tC.
+         ** apply:eqf_tT_tT.
+    * constructor.
+      -- apply:(rl_t_C (ft_r st)).
+      -- apply:ft_rT.
+      -- apply:ft_r.
+      -- cbn .
+         move:(ft_r su).
+         apply:transport.
+         ++ apply:pt_eq.
+            ** apply:eqf_tC_tC.
+            ** apply:eqf_tT_tT.
+            ** apply:JMeq_sym.
+               apply:JMeq_transport2.
+- destruct wt.
+  + specialize (semV _ _ _ wΓ wA w).
+    econstructor.
+    * constructor.
+      exact:(fV_r semV).
+  + specialize (semS _ _ _ wΓ w w1).
+    move/semT:(w0).
+    move/(_ w) => IHA.
+    assert ( e : fT_C IHA = fS_Δ semS).
+    {
+      apply:rl_hpC.
+      - apply:(rl_T_C (fT_r IHA)).
+      - apply:(rl_S_C2 (fS_r semS)).
+    }
+    econstructor.
+    * constructor; revgoals.
+      -- apply:(fS_r semS).
+      -- assert (h' : rl_T fibT w w0 (mkpT (eq_rect _ (@rT T) (fT_T IHA) _ e))).
+         { move: (fT_r IHA).
+           apply:transport.
+           move:(fT_T IHA).
+           pattern (fT_C IHA),e.
+           by apply:J.
+         }
+         exact:h'.
+      -- apply:(rl_S_C2 (fS_r semS)).
+      -- apply:(rl_S_C1 (fS_r semS)).
+- destruct wx.
+  +
+    have e : wΓ = w_astar by   apply:WC_hp.
+    subst.
+    have e : wA = w_star w_astar by   apply:WTy_hp.
+    subst.
+    repeat econstructor.
+  + (* weakening *)
+    rename w into wu.
+    move/semt:(wu) => IHu.
+    move/semV:(wx) => IHx.
+    rename wA into wB.
+    assert ( wA : Γ ⊢ A).
+    { abstract (by inversion wΓ).  }
+    assert ( wΓ' :WC Γ).
+    { abstract (by inversion wΓ).  }
+    have e : wΓ = w_ext wΓ' wA wu by apply:WC_hp.
+    subst.
+    specialize (IHx wΓ' (WVar_Ty wΓ' wx)).
+    specialize (IHu wΓ' wA).
+    have rx := fV_r IHx.
+    have rA := fV_rT IHx.
+    have ru := ft_r IHu.
+    have eΓ : fV_C IHx = ft_C IHu.
+    {
+      apply:rl_hpC.
+      -  exact:(rl_V_C rx).
+      -  exact:(rl_t_C ru).
+    }
+    have rAu : rl_T fibT wΓ' wA {| pT_C := fV_C IHx; pT_T :=
+                                                       eq_rect_r (@rT T) (ft_T IHu) eΓ |}.
+    {
+      move:(ft_rT IHu).
+      apply:transport.
+      move:(ft_T IHu).
+      pattern (ft_C IHu),eΓ.
+        by apply:J_r.
+    }
+    have ru' :
+      rl_t fibT wΓ' wA wu
+           {|
+             pt_C := fV_C IHx;
+             pt_T := eq_rect_r (@rT T) (ft_T IHu) eΓ;
+             pt_t := transport2 (Logic.eq_sym eΓ)
+                                (JMeq_sym (JMeq_eq_rect_r (ft_T IHu) eΓ)) (ft_t IHu) |}.
+    {
+      move:(ft_r IHu).
+      apply:transport.
+      move:(ft_t IHu).
+      move:(ft_T IHu).
+      pattern (ft_C IHu),eΓ.
+      apply:J_r.
+      cbn.
+      intros.
+      cbn.
+      rewrite JMeq_eq_refl.
+      reflexivity.
+    }
+
+
+    (* destruct IHx,IHu; subst; simpl in *. *)
+    (* subst. *)
+    econstructor.
+    * apply:rl_vwk; last by apply:rx.
+      -- rewrite eΓ. exact:(rl_t_C ru).
+      -- exact:rAu.
+      -- move:ru.
+         apply:transport.
+         symmetry.
+         apply:pt_eq => //.
+         ++ apply:JMeq_eq_rect_r.
+         ++ apply:JMeq_transport2 => //.
+            apply:JMeq_sym.
+            apply:JMeq_eq_rect_r.
+
+      -- assumption.
+  + rename w into wu.
+    assert ( wA' : Γ ⊢ A).
+    { abstract (by inversion wΓ).  }
+    assert ( wΓ' :WC Γ).
+    { abstract (by inversion wΓ).  }
+    move/semt:(wu).
+    move/(_ wΓ' wA') => IHu.
+    have e : wΓ = w_ext wΓ' wA' wu by apply:WC_hp.
+    subst.
+    have ru := ft_r IHu.
+    (* have r :  rl_C fibT wΓ' (ft_C IHu) *)
+
+    econstructor.
+    * constructor; last by apply:ru.
+      -- exact:(rl_t_C ru).
+      -- exact:(ft_rT IHu).
+  + rename w into wu.
+    inversion wΓ; subst.
+    rename X0 into wA'.
+    rename X into wΓ'.
+    clear X1.
+    move/semt:(wu).
+    move/(_ wΓ' wA') => IHu.
+    have e : wΓ = w_ext wΓ' wA' wu by apply:WC_hp.
+    subst.
+    have ru := ft_r IHu.
+
+    inversion wA; subst.
+    rename X into wAe.
+    rename X1 into wue.
+    have e : wA = w_ar wAe (w_va (w_v1 wu)) wue by apply:WTy_hp.
+    subst.
+    (* have r :  rl_C fibT wΓ' (ft_C IHu) *)
+
+    econstructor.
+    * apply:rl_v0 ; last by apply:ru.
+      -- exact:(rl_t_C ru).
+      -- exact:(ft_rT IHu).
+- destruct wσ.
+  + move/semt:(w) => /(_ wΓ (w_star wΓ)) IHt.
+    have e : wΔ = w_astar by apply:WC_hp.
+    have rt := (ft_r IHt).
+
+    subst wΔ.
+    econstructor.
+    constructor.
+    * exact:(rl_t_C rt).
+    * simpl.
+      apply:tp_rTm1; last by exact:rt.
+      -- reflexivity.
+      -- unshelve eapply pt_eq1.
+         ++   apply:π_eq_pTη.  
+              apply:rl_hpT.
+              ** constructor.
+                 exact:(rl_t_C rt).
+              ** apply :(ft_rT IHt).
+         ++  apply eq_rect_inv.
+  + 
+    have wΔ' : WC Δ by inversion wΔ.
+    move/semS:(wσ) => /(_ wΓ wΔ') IHσ.
+    move/semT:(w) => /(_  wΔ') IHA.
+    move/semt:(w0) => /(_  wΔ' w) IHu.
+    have wAσ := WTy_sb wΓ wΔ' wσ w.
+    have wuσ := Wtm_sb wΓ wΔ' wσ w0.
+    move/semt:(w2) => /(_  wΓ (w_ar wAσ w1 wuσ)) IHf.
+    move/semt:(w1) => /(_  wΓ wAσ) IHt.
+    have e : wΔ = w_ext wΔ' w w0 by apply:WC_hp.
+    subst.
+    have rσ := fS_r IHσ.
+    have rA := fT_r IHA.
+    have ru := ft_r IHu.
+    have rt := ft_r IHt.
+    have rf := ft_r IHf.
+    have esΔ : fT_C IHA = fS_Δ IHσ.
+    {
+      apply:rl_hpC.
+      - exact:(rl_T_C rA).
+      - exact:(rl_S_C2 rσ).
+    }
+  
+    have esΔ' : fS_Δ IHσ = ft_C IHu.
+    {
+      apply:rl_hpC.
+      - exact:(rl_S_C2 rσ).
+      - exact:(rl_t_C ru).
+    }
+    have e :   fS_Γ IHσ  = ft_C IHt.
+    {
+      apply:rl_hpC.
+      - exact:(rl_S_C1 rσ).
+      - apply:(rl_t_C rt).
+    }
+
+
+    destruct IHσ,IHu,IHA,IHf,IHt; simpl in *; subst.
+    have ft_rT2 := rl_t_Tη ft_r2.
+    have ft_rT1 := rl_t_Tη ft_r1.
+    have e :   fT_T0  = ft_T0.
+    { apply:π_eq_pTη; apply:rl_hpT.
+      - eassumption.
+      - apply:rl_t_Tη.
+        eassumption.
+    }
+    subst.
+    have e :   ft_C1  = ft_C2.
+    {
+      apply:rl_hpC.
+      - exact:(rl_t_C rf).
+      - exact:(rl_t_C rt).
+    }
+    subst.
+    have e : ft_T2 = r_sbT fS_S0 ft_T0.
+    {
+      apply:π_eq_pTη.
+      apply:rl_hpT; last first.
+      + apply:(rl_sbT (pA := mkpT ft_T0)); eassumption.
+      + apply:tp_rT1; last by exact:ft_rT2.
+        * reflexivity.
+        * reflexivity.
+    }
+    subst.
+
+  (* {| pt_C := fS_Γ0; pt_T := r_sbT fS_S0 (eq_rect_r rT ft_T0 (erefl ft_C0)); pt_t := ?Goal2 |} = *)
+  (* {| pt_C := ft_C2; pt_T := ft_T2; pt_t := ft_t2 |} *)
+
+    econstructor.
+    apply:rl_to_ext.
+    * apply:(rl_S_C1 rσ).
+    * apply:(rl_S_C2 rσ).
+    * simpl.
+      apply:tp_rT1; last by exact:rA.
+      -- reflexivity.
+      -- unshelve eapply pT_eq1.
+         ++ now symmetry.
+         ++ reflexivity.
+    * simpl.
+
+      apply:tp_rTm1; last by exact:ru.
+      -- reflexivity.
+      -- reflexivity.
+    * simpl. exact:rσ.
+    * simpl.
+      apply:tp_rTm1; last by exact:ft_r2.
+      -- reflexivity.
+      -- unshelve eapply pt_eq1.
+         ++ reflexivity.
+         ++  reflexivity.
+            (* apply:eq_rect_inv. *)
+    * simpl.
+      apply:tp_rTm1; last by exact:rf.
+      -- reflexivity.
+      -- unshelve eapply pt_eq1.
+         ++ cbn.
+            apply:π_eq_pTη.
+            apply:rl_hpT; last first.
+            **  eassumption.
+            ** cbn.
+               apply:rl_ar.
+               --- apply :(rl_T_C ft_rT1).
+               --- assumption.
+               --- exact:rt. 
+               --- apply:tp_rTm1; last first.
+                   +++ apply: (rl_sbt (pt := mkpt ft_t0)); eassumption.
+                   +++ reflexivity.
+                   +++ reflexivity.
+         ++ cbn.
+            apply:eq_rect_inv.
+    Unshelve.
+    assumption.
+    assumption.
+Defined.
+
+
+End TypeRl.
