Modules/TypeSystem/decl.v
@@ -1,18 +1,14 @@
+
 Require Import ssreflect ssrfun ssrbool .
 
-From Modules Require Import Syntax libhomot lib.
+From Modules Require Import Syntax libhomot lib gtype.
 Require Import Coq.Logic.JMeq.
+
 Set Bullet Behavior "Strict Subproofs".
 
 Set Implicit Arguments.
 Unset Strict Implicit.
 Unset Printing Implicit Defensive.
-
-CoInductive GType :=
-  Gtyp { ob : Type ;
-         hom : ob -> ob -> GType }.
-
-Notation "∣ A ∣" := (ob A) (at level 99).
 
 Class Decl {P : PreSyntax} {S : Syntax P} :=
   { dC : forall Γ, WC Γ -> Type;
@@ -23,7 +19,6 @@ Class Decl {P : PreSyntax} {S : Syntax P} :=
             dC wΔ
   }.
 
-
 Definition extΣ_G (Γ : Type) (A : Γ -> GType) (u : forall γ, ∣ A γ ∣) :=
   { δ : { γ : Γ & ∣ A γ ∣ } & ∣ hom δ..2 (u δ..1) ∣ }.
 
@@ -31,14 +26,3 @@ Notation "⟦ X ⟧C" := (dC X).
 Notation "⟦ X ⟧T" := (dTy X).
 Notation "⟦ X ⟧t" := (dTm X).
 Notation "⟦ X ⟧S" := (dS X).
-
-CoFixpoint G_of_T (T : Type) : GType.
-  unshelve econstructor.
-  - exact:T.
-  - move => a b.
-    apply:G_of_T.
-    exact: (a =h b).
-Defined.
-(* Notation "∣ X ∣" := (ob X). *)
-
-
