Modules/TypeSystem/gtype.v
@@ -1,0 +1,29 @@
+Require Import ssreflect ssrfun ssrbool .
+
+From Modules Require Import Syntax libhomot lib.
+Require Import Coq.Logic.JMeq.
+Set Bullet Behavior "Strict Subproofs".
+
+Set Implicit Arguments.
+Unset Strict Implicit.
+Unset Printing Implicit Defensive.
+
+CoInductive GType :=
+  Gtyp { ob : Type ;
+         hom : ob -> ob -> GType }.
+
+Notation "∣ A ∣" := (ob A) (at level 99).
+
+
+
+
+CoFixpoint G_of_T (T : Type) : GType.
+  unshelve econstructor.
+  - exact:T.
+  - move => a b.
+    apply:G_of_T.
+    exact: (a =h b).
+Defined.
+(* Notation "∣ X ∣" := (ob X). *)
+
+
